\subsection{含有$ax+b$的积分}
\begin{enumerate}
	\item $\int \frac{dx}{ax+b}=\frac{1}{a}ln|ax+b|+C$
	
		推导：
		\begin{equation}
			\label{eq:adv1}
			\begin{split}
				\int \frac{dx}{ax+b} &=\frac{1}{a}\frac{d(ax+b)}{ax+b}\\
				&=\frac{1}{a}ln|ax+b|+C
			\end{split}
		\end{equation}
		\item $\int(ax+b)^{\mu}dx=\frac{1}{a(u+1)}(ax+b)^{\mu+1}$
		推导：
	
			\begin{align}
				\label{eq:adv2}
				\int(ax+b)^{\mu}dx&=\frac{1}{a}\int(ax+b)^{\mu}d{ax+b}\\
				&=\frac{1}{a(u+1)}(ax+b)^{\mu+1}\quad(\mu\neq -1)
			\end{align}

			\item $\int\frac{x}{ax+b}dx = \frac{1}{a^2}(ax+b-bln|ax+b|)+C$
			推导：
			\begin{align}
				\label{eq:adv3}
				\int\frac{x}{ax+b}dx &= \frac{1}{a^2}\int\frac{ax}{ax+b}dax\\
				&=\frac{1}{a^2}\int\frac{ax+b-b}{ax+b}dax\\ 
				&=\frac{1}{a^2}\int1d(ax+b)-\frac{b}{a^2}\int\frac{1}{ax+b}d(ax+b)\\
				&=\frac{1}{a^2}(ax+b)-\frac{b}{a^2}ln(ax+b)+C\\
				&=\frac{1}{a^2}(ax+b-bln|ax+b|)+C
			\end{align}
		\item $\int\frac{x^2}{ax+b}dx=\frac{1}{a^3}\left[\frac{1}{2}(ax+b)^2-2b(ax+b)+b^2ln|ax+b|\right]+C$
		推导：
		\begin{equation}
			\label{eq:adv4}
			\begin{split}
				\int\frac{x^2}{ax+b}dx&=\frac{1}{a}\int\frac{ax^2}{ax+b}dx\\ 
				&= \frac{1}{a}\int xdx-\frac{b}{a}\int \frac{x}{ax+b}dx\\ 
				&= \frac{x^2}{2a}-\frac{b}{a^3}(ax+b-bln|ax+b|)+C
			\end{split}
		\end{equation}
		\item $\int\frac{dx}{x(ax+b)}=-\frac{1}{b}ln|\frac{ax+b}{x}|+C$
		推导：
		\begin{equation}
			\label{eq:adv5}
			\begin{split}
				\int\frac{dx}{x(ax+b)}&=\frac{1}{b}(\frac{1}{x}-\frac{a}{ax+b})dx\\ 
				&=\frac{ln|x|}{b}-\frac{ln|ax+b|}{b}=-\frac{1}{b}ln|\frac{ax+b}{x}|+C
			\end{split}
		\end{equation}
		\item $\int\frac{dx}{x^2(ax+b)}=-\frac{1}{bx}+\frac{a}{b^2}ln{|\frac{ax+b}{x}|}+C$
		推导：
		\begin{equation}
			\begin{split}
				\int\frac{dx}{x^2(ax+b)} &= \int \frac{\frac{-a}{b^2}x+\frac{1}{b}}{x^2}+\frac{a^2}{b^2}\frac{1}{ax+b}dx\\ 
				&=-\frac{1}{bx}+\frac{a}{b^2}ln(|\frac{ax+b}{x}|)+C
			\end{split}
		\end{equation}
		\item $\int\frac{x}{(ax+b)^2}dx=\frac{1}{a^2}(ln|ax+b|+\frac{b}{ax+b})+C$
		推导：
		\begin{equation}
			\label{eq:adv8}
			\begin{split}
				\int\frac{x}{(ax+b)^2}dx&=\frac{1}{a^2}\int \frac{ax+b-b}{(ax+b)^2}d{(ax+b)}\\ 
				&=\frac{1}{a^2}\left(ln|ax+b|+\frac{b}{ax+b}\right)
			\end{split}
		\end{equation}
		\item $\int\frac{x^2}{(ax+b)^2}dx=\frac{1}{a^3}\left(ax+b-2bln|ax+b|-\frac{b^2}{ax+b}\right)+C$
		推导：
		\begin{equation}
			\begin{split}
				\int\frac{x^2}{(ax+b)^2}dx&=\frac{1}{a^3}\left(\int 1-2ab\frac{x}{(ax+b)^2}-\frac{b^2}{(ax+b)^2}\right)d{(ax+b)}\\ 
				&=\frac{1}{a^3}\left(ax+b -\frac{2b}{a}(ln|ax+b|)\cdot a-\frac{2b}{a}(\frac{b}{ax+b})\cdot a\right)-\\ 
				&\int \frac{b^2}{ax+b}d{(ax+b)}\\ 
				&=\frac{1}{a^3}\left(ax+b-2bln|ax+b|-\frac{b^2}{ax+b}\right)+C
			\end{split}
		\end{equation}
		\item $\int\frac{dx}{x(ax+b)^2}=\frac{1}{b(ax+b)}-\frac{1}{b^2}ln|\frac{ax+b}{x}|+C$
		推导：
		\begin{equation}
			\begin{split}
				\int\frac{dx}{x(ax+b)^2}&=-\frac{1}{a}\int \frac{1}{x}d{\frac{1}{ax+b}}\\ 
				&=-\frac{1}{a}\left(\frac{1}{(ax+b)x}+\int\frac{1}{x^2(ax+b)}\right)\\ 
				&=-\frac{1}{a}\left(\frac{1}{(ax+b)x}-\frac{1}{bx}+\frac{a}{b^2}ln{|\frac{ax+b}{x}|}\right)\\ 
				&=\frac{1}{b(ax+b)}-\frac{1}{b^2}ln|\frac{ax+b}{x}|+C
			\end{split}
		\end{equation}

\end{enumerate}
\subsection{含有$\sqrt{{ax+b}}的积分$}
\begin{enumerate}
	\item $\int \sqrt{ax+b}dx=\frac{2}{3a}\sqrt{\left(ax+b\right)^3}+C$
	推导：
	\begin{equation}
		\begin{split}
			\int \sqrt{ax+b}dx&= \frac{1}{a}\int \frac{\left(ax+b\right)^{1/2}}d(ax+b)\\ 
			&=\frac{2}{3} \sqrt{\left(ax+b\right)^3}
		\end{split}
	\end{equation}
	\item $\int x\sqrt{ax+b}dx=\frac{2}{15a^2}(3ax-2b)\sqrt{\left(ax+b\right)^3}+C$
	推导：
	\begin{equation}
		\begin{split}
			\int x\sqrt{ax+b}dx&=\frac{1}{a^2}\int(ax+b-b)\sqrt{ax+b}d{ax}\\ 
			&= \frac{1}{a^2}\left(ax+b\right)^{\frac{3}{2}}-\frac{2b}{3}(ax+b)^{\frac{3}{2}}d{ax}\\ 
			&=\frac{1}{a^2}\left[\frac{2}{5}\left(ax+b\right)^{\frac{5}{2}}-\frac{2b}{3}\left(ax+b\right)^{\frac{3}{2}}\right]+C\\ 
			&= \frac{2}{15a^2}(3ax-2b)\sqrt{\left(ax+b\right)^3}+C
		\end{split}
	\end{equation}
	\item $\int x^2\sqrt{ax+b}dx=\frac{2}{105a^3}(15a^2x^2-12abx+8b^2)\sqrt{\left(ax+b\right)^3}+C$
	推导：
	\begin{equation}
		\begin{split}
			\int x^2\sqrt{ax+b}dx &=\frac{1}{a^3}\int (ax+b)^2\sqrt{ax+b}-2abx\sqrt{ax+b}-b^2\sqrt{ax+b}d{ax} \\
				&=\frac{1}{a^3}\left(\frac{2}{7}(ax+b)^{\frac{7}{2}}-2ab\frac{2}{15a}(3ax-2b)\sqrt{\left(ax+b\right)^3}-\frac{2b^2}{3}(ax+b)^{\frac{3}{2}}\right)+C\\ 
				&=\frac{2\sqrt{\left(ax+b\right)^3}}{105a^3}\left(15(ax+b)^2-14b(3ax-2b)-35b^2\right)+C\\ 
				&=\frac{2\sqrt{(15a^2x^2-12abx+8b^2)}}{105a^3}\left(ax+b\right)^3+C
		\end{split}
	\end{equation}
	\item $\int \frac{x}{\sqrt{ax+b}}dx=\frac{2}{3a^2}(ax-2b)\sqrt{ax+b}+C$
	推导：
	\begin{equation}
		\begin{split}
			\int \frac{x}{\sqrt{ax+b}}dx &=\int \frac{1}{a^2}\frac{ax+b-b}{\sqrt{ax+b}}d{ax} \\ 
			&=\frac{1}{a^2}\left(\int \sqrt{ax+b}-(ax+b)^{-\frac{1}{2}})d{ax+b}\right) \\ 
			&=\frac{1}{a^2}\left(\frac{2}{3}(ax+b)^{1/2}(ax+b)-2b\right)+C \\ 
			&=\frac{2}{3a^2}\left(\frac{2}{3}(ax+b)^{1/2}(ax+b)-3b\right)+C \\ 
			&=\frac{2}{3a^2}(ax-2b)\sqrt{ax+b}+C
		\end{split}
	\end{equation}
	\item $\int \frac{x^2}{\sqrt{ax+b}}dx=\frac{2}{15a^3}(3a^2x^2-4abx+8b^2)\sqrt{ax+b}+C$
	推导：
	\begin{equation}
		\begin{split}
			\int \frac{x^2}{\sqrt{ax+b}}dx&=\frac{1}{a^3}(\frac{(ax+b)^2-2abx-b^2}{\sqrt{ax+b}})dax\\ 
			&=\frac{1}{a^3}\left(\frac{2}{5}\left(ax+b\right)^{\frac{5}{2}}\right)-2ab \frac{2}{3a}(ax-2b)\sqrt{ax+b}-2b^2\sqrt{ax+b}+C\\ 
			&=\frac{2}{15a^3}\left(3(ax)^2+6abx+3b^2-10abx+20b^2-15b^2\right)\sqrt{ax+b}+C\\ 
			&=\frac{2}{15a^3}\left(3(ax)^2-4abx+8b^2\right)\sqrt{ax+b}+C
		\end{split}
	\end{equation}
	\item \begin{equation}
		\int \frac{dx}{x\sqrt{ax+b}}dx=\begin{cases}
	\frac{1}{\sqrt{b}}ln|\frac{\sqrt{ax+b}-\sqrt{b}}{\sqrt{ax+b}+\sqrt{b}}|+C\quad (b>0)\\
	\frac{2}{\sqrt{-b}}arctan\sqrt{\frac{ax+b}{-b}}+C\quad (b<0)
	\end{cases}
\end{equation}
	\item $\int \frac{dx}{x^2\sqrt{ax+b}}=-\frac{\sqrt{ax+b}}{bx}-\frac{a}{2b}\int\frac{dx}{x\sqrt{ax+b}}$
	推导：
	\begin{equation}
		\begin{split}
			\int \frac{dx}{x^2\sqrt{ax+b}} &=\int \frac{dx}{x\sqrt{ax+b}}\frac{1}{x}
		\end{split}
	\end{equation}
	\item $\int \frac{\sqrt{ax+b}}{x}dx=2\sqrt{ax+b}+b\int\frac{dx}{x\sqrt{ax+b}}$
	推导：
	\begin{equation}
		\begin{split}
			\int \frac{\sqrt{ax+b}}{x}dx&=\int \frac{\sqrt{ax+b}}{\sqrt{x}}d{2\sqrt{x}}\\ 
			&=2\sqrt{ax+b}+\int b\sqrt{\frac{x}{ax+b}}\cdot\frac{1}{x^2}\cdot\sqrt{x}d{x}\\ 
			&=2\sqrt{ax+b}+b\int\frac{dx}{x\sqrt{ax+b}}dx
		\end{split}
	\end{equation}
	\item $\int \frac{\sqrt{ax+b}}{x^2}dx=-\frac{\sqrt{ax+b}}{x}+\frac{a}{2}\int \frac{dx}{x\sqrt{ax+b}}$
	推导：
	\begin{equation}
		\begin{split}
			\int \frac{\sqrt{ax+b}}{x^2}dx&=-\int \sqrt{ax+b}d\frac{1}{x}\\ 
			&=\frac{\sqrt{ax+b}}{x}+\frac{a}{2}\int \frac{dx}{x\sqrt{ax+b}}dx
		\end{split}
	\end{equation}
\end{enumerate}
\subsection{含有$x^2\pm a^2$}
\begin{enumerate}
	\item $\int \frac{dx}{x^2+a^2}=\frac{1}{a}arctan\frac{x}{a}+C$
	推导：
	\begin{equation}
		\begin{split}
			\int \frac{dx}{x^2+a^2}&=\int \frac{1}{a}\frac{d\frac{x}{a}}{{\frac{x}{a}}^2+1^2}\\
			&=\frac{1}{a}arctan(\frac{x}{a})+C
		\end{split}
	\end{equation}
	\item $\int\frac{dx}{\left(x^2+a^2\right)^n}=\frac{x}{2(n-1)a^2(x^2+a^2)^{n-1}}+\frac{2n-3}{2(n-1)a^2}\int\frac{dx}{(x^2+a^2)^{n-1}}$
	\item $\int \frac{dx}{x^2-a^2}=\frac{1}{2a}ln|\frac{x-a}{x+a}|+C$
	\begin{equation}
		\begin{split}
			\int \frac{dx}{x^2-a^2}&=\frac{1}{2a}\int \frac{1}{x-a}-\frac{1}{x+a}dx\\ 
			&=\frac{1}{2a}ln|\frac{x-a}{x+a}|\
		\end{split}
	\end{equation}
\end{enumerate}
\subsection{含有$ax^2+b (a>0)的积分$}
\begin{enumerate}
	\item $\int \frac{dx}{ax^2+b}=\begin{cases}
	\frac{1}{\sqrt{ab}}arctan\sqrt{\frac{a}{b}}x+C \quad (b>0)\\ 
	\frac{1}{2\sqrt{-ab}}ln|\frac{\sqrt{a}x-\sqrt{-b}}{\sqrt{a}x+\sqrt{-b}}|+C
	\end{cases}$

	推导：
	\begin{align}
			\int \frac{dx}{ax^2+b}&=\frac{1}{\sqrt{a}}\int\frac{1}{x^2+\frac{b}{a}}dx\\ 
			&=
				\begin{cases}
					\frac{1}{a}\int\frac{1}{x^2+\left(\sqrt{\frac{b}{a}}\right)^2}dx = \frac{1}{a}\left(\sqrt{\frac{a}{b}}\right)arctan\sqrt{\frac{a}{b}}x+C=\frac{1}{\sqrt{ab}}arctan\sqrt{\frac{a}{b}}x+C \quad (b>0)\\ 
					\frac{1}{a}\int \frac{1}{x^2-\left(\sqrt{\frac{-b}{a}}\right)^2}dx = \int \frac{1}{2a}\cdot\sqrt{\frac{a}{-b}}ln|\frac{x-\sqrt{\frac{b}{a}}}{x+\sqrt{\frac{b}{a}}}|dx=\frac{1}{2\sqrt{-ab}}ln|\frac{\sqrt{a}x-\sqrt{-b}}{\sqrt{a}x+\sqrt{-b}}|+C
				\end{cases}
	\end{align}
	\item $\int \frac{x}{ax^2+b}dx=\frac{1}{2a}ln|ax^2+b|+C$
	推导：
	\begin{equation}
		\begin{split}
			\int \frac{x}{ax^2+b}dx&=\frac{1}{2a}\int\frac{1}{ax^2+b}d{ax^2+b}=\frac{1}{2a}ln|ax^2+b|+C
		\end{split}
	\end{equation}
	\item $\int\frac{x^2}{ax^2+b}dx=\frac{x}{a}-\frac{b}{a}\int\frac{ax}{ax^2+b}$
	\item $\int\frac{dx}{x(ax^2+b)}=\frac{1}{2b}\ln\frac{x^2}{|ax^2+b|}+C$
	\item $\int\frac{dx}{x^2(ax^2+b)}=-\frac{1}{bx}-\frac{a}{b}\int\frac{dx}{ax^2+b}$
	\item $\int\frac{dx}{x^3(ax^2+b)}=\frac{a}{2b^2}ln\frac{|ax^2+b|}{x^2}-\frac{1}{2bx^2}+C$
	\item $\int\frac{dx}{(ax^2+b)^2}=\frac{x}{2b(ax^2+b)}+\frac{1}{b}\int\frac{dx}{ax^2+b}$
\end{enumerate}
\subsection{含有$ax^2+bx+c(a>0)$的积分}
\begin{itemize}
\item $\int\frac{dx}{ax^2+bx+c}=\begin{cases}\frac{2}{\sqrt{4ac-b^2}}arctan\frac{2ax+b}{\sqrt{4ac-b^2}+C}\quad (b^2<4ac)\\\frac{1}{\sqrt{b^2-4ac}}ln|\frac{2ax+b-\sqrt{b^2-4ac}}{2ax+b+\sqrt{b^2-4ac}}|+C\quad (b>4ac)\end{cases}$
\item $\int\frac{x}{ax^2+bx+c}dx=\frac{1}{2a}\ln|ax^2+bx+c|-\frac{b}{2a}\int\frac{dx}{ax^2+bx+c}$
\end{itemize}
\subsubsection{含有$\sqrt{x^2+a^2}$}
\begin{itemize}
	\item $\int \frac{dx}{\sqrt{x^2+a^2}}=arsh\frac{x}{a}+C_1=ln(x+\sqrt{x^2+a^2})+C$
	\item $\int \frac{dx}{\sqrt{(x^2+a^2)^3}}=\frac{x}{a^2\sqrt{x^2+a^2}}+C$
	\item $\int \frac{x}{\sqrt{x^2+a^2}}=\sqrt{x^2+a^2}+C$
	\item $\int\frac{x}{\sqrt{(x^2+a^2)^3}}dx=-\frac{1}{\sqrt{x^2+a^2}}+C$
	\item $\int\frac{x^2}{\sqrt{x^2+a^2}}dx=\frac{x}{2}\sqrt{x^2+a^2}-\frac{a^2}{2}ln\left(x+\sqrt{x^2+a^2}\right)+C$
	\item $\int \frac{x^2}{\sqrt{\left(x^2+a^2\right)^3}}=-\frac{x}{\sqrt{x^2+a^2}}+ln\left(x+\sqrt{x^2+a^2}\right)+C$
	\item $\int\frac{dx}{x\sqrt{x^2+a^2}}=\frac{1}{a}\ln\frac{\sqrt{x^2+a^2}-a}{|x|}+C$
	\item $\int\frac{dx}{x^2\sqrt{x^2+a^2}}=-\frac{x^2+a^2}{a^2x}+C$
	\item $\int\sqrt{x^2+a^2}dx=\frac{x}{2}\sqrt{x^2+a^2}+\frac{a^2}{2}\ln(x+\sqrt{x^2+a^2})+C$
	\item $\int \sqrt{\left(x^2+a^2\right)^3}dx=\frac{x}{8}(2x^2+5a^2)\sqrt{x^2+a^2}+\frac{3}{8}a^4ln(x+\sqrt{x^2+a^2})+C$
	\item $\int x\sqrt{x^2+a^2}dx=\frac{1}{3}\sqrt{\left(x^2+a^2\right)^3}+C$
	\item $\int x^2\sqrt{x^2+a^2}dx=\frac{x}{8}(2x^2+a^2)\sqrt{x^2+a^2}-\frac{a^4}{8}\ln(x+\sqrt{x^2+a^2})+C$
	\item $\int\frac{\sqrt{x^2+a^2}}{x}dx=\sqrt{x^2+a^2}+aln\frac{\sqrt{x^2+a^2}-a}{|x|}+C$
	\item $\int\frac{\sqrt{x^2+a^2}}{x^2}dx=-\frac{\sqrt{x^2+a^2}}{x}+ln(x+\sqrt{x^2+a^2})+C$
\end{itemize}
\subsection{含有$\sqrt{x^2-a^2}(a>0)$的积分}
\begin{itemize}
	\item $\int\frac{dx}{\sqrt{x^2-a^2}}=\frac{x}{|x|}arch\frac{|x|}{a}+C_1=ln|x+\sqrt{x^2-a^2}|+C$
	\item $\int\frac{dx}{\sqrt{\left(x^2-a^2\right)^3}}=-\frac{x}{a^2\sqrt{x^2-a^2}}+C$
	\item $\int \frac{x}{x^2-a^2}dx=\sqrt{x^2-a^2}+C$
	\item $\int\frac{x}{\sqrt{(x^2-a^2)}}dx=-\frac{1}{\sqrt{x^2-a^2}}+C$
	\item $\int\frac{x^2}{\sqrt{x^2-a^2}}dx=\frac{x}{2}\sqrt{x^2-a^2}+\frac{a^2}{2}ln|x+\sqrt{x^2-a^2}|+C$
	\item $\int\frac{x^2}{\sqrt{\left(x^2-a^2\right)}}x=-\frac{x}{\sqrt{x^2-a^2}}+ln|x+\sqrt{x^2-a^2}|+C$
	\item $\int\frac{dx}{x\sqrt{x^2-a^2}}=\frac{1}{a}arccos\frac{a}{|x|}+C$
	\item $\int\frac{dx}{x^2\sqrt{x^2-a^2}}=\frac{(x^2-a^2)}{a^2x}+C$
	\item $\int\sqrt{x^2-a^2}dx=\frac{x}{2}\sqrt{x^2-a^2}-\frac{a}{2}ln|x+\sqrt{x^2-a^2}|+C$
	\item $\int\sqrt{\left(x^2-a^2\right)^3}=\frac{x}{8}(2x^2-5a^2)\sqrt{x^2-a^2}+\frac{3}{8}a^4\ln|x+\sqrt{x^2-a^2}|+C$
	\item $\int x\sqrt{x^2-a^2}dx=\frac{1}{3}\sqrt{\left(x^2-a^2\right)^3}+C$
	\item $\int x^2\sqrt{x^2-a^2}dx=\frac{x}{8}(2x^2-a^2)\sqrt{x^2-a^2}-\frac{a^4}{8}\ln|x+\sqrt{x^2-a^2}|+C$
	\item $\int \frac{\sqrt{x^2-a^2}}{x}dx=\sqrt{x^2-a^2}-aarccos\frac{a}{|x|}+C$
	\item $\int\frac{\sqrt{x^2-a^2}}{x^2}dx=-\frac{\sqrt{x^2-a^2}}{x}+\ln|x+\sqrt{x^2-a^2}|+C$
\end{itemize}
\subsection{含有$\sqrt{a^2-x^2}(a>0)$的积分}
\begin{itemize}
	\item $\int\frac{dx}{\sqrt{a^2}-x^2}=arcsin\frac{x}{a}+C$
	\item $\int csc^2xdx=-cotx+C$
	\item $\int \sec x \tan xdx=\sec x+C$
	\item $\int\csc x \cot xdx = =-\csc x+c$
	\item $\int \sin^2x=\frac{x}{2}-\frac{1}{4}\sin2x+C$
	\item $\int \cos^2dx=\frac{x}{2}+\frac{1}{4}\sin2x+C$
	\item $\int \sin^nxdx = -\frac{1}{n}\sin^{n-1}\cos x+\frac{n-1}{n}\int\sin^{n-1}xdx$
	\item $\int \cos^nxdx = \frac{1}{n}\cos^{n-1}x\sin x+\frac{n-1}{n}\int\cos^{n-2}dx$
	\item $\int \frac{dx}{\sin^nx}=-\frac{1}{n-1}\cdot \frac{\cos x}{sin^{n-1}}+\frac{n-2}{n-1}\int\frac{dx}{\sin^{n-2}x}dx$
	\item $\int \frac{dx}{cos^nx}=\frac{1}{n-1}\cdot \frac{\sin x}{\cos^{n-1}(x)}+\frac{n-2}{n-1}\int \frac{dx}{\cos^{n-2}x}$
	\item $\int \cos^mx\sin^xdx=\frac{1}{m+n}cos^{m-1}xsin^{n+1}x+\frac{m-1}{m+n}\int\cos^{m-2}x\sin^nxdx=-\frac{1}{m+n}cos^{m+1}xsin^{n-1}x+\frac{m-1}{m+n}\int cos^mxsin^{n-2}xdx$
	\item $\int \sin ax\cos bxdx = -\frac{1}{2(a+b)}\cos(a+b)x-\frac{1}{2(a-b)}cos(a-b)x+C$
	\item $\int \sin ax\sin bxdx=-\frac{1}{2(a+b)}\sin(a+b)x+\frac{1}{2(a-b)}\sin(a-b)x+C$
	\item $\int \cos ax \cos bxdx=\frac{1}{2(a+b)}\sin(a+b)x+\frac{1}{2(a-b)}\sin(a-b)x+C$
	\item $\int \frac{dx}{a+b\sin x}=\frac{2}{\sqrt{a^2-b^2}}arctan\frac{a\tan\frac{x}{2}+b}{\sqrt{a^2-b^2}}+C(a^2>b^2)$
	\item $\int \frac{dx}{a+b\sin x}=\frac{1}{\sqrt{b^2-a^2}}ln|\frac{a\tan\frac{x}{2}+b-\sqrt{b^2-a^2}}{a\tan\frac{x}{2}+b-\sqrt{b^2-a^2}}|+C(a^2<b^2)$
	\item $\int\frac{dx}{a+b\cos x}=\frac{2}{a+b}\sqrt{\frac{a+b}{a-b}}archtan\left(\sqrt{\frac{a-b}{a+b}}\tan\frac{x}{2}\right)+C(a^2>b^2)$
	\item $\int \frac{dx}{a+b\cos x}=\frac{1}{a+b}\sqrt{\frac{a+b}{a-b}}\ln|\frac{\tan\frac{x}{2}+\sqrt{\frac{a+b}{a-b}}}{\tan\frac{x}{2}-\sqrt{\frac{a+b}{a-b}}}+C(a^2<b^2)| $
	\item $\int \frac{dx}{a^2cos^2x+b^2cos^2x}=\frac{1}{ab}\arctan\left(\frac{b}{a}\tan x\right)+C$
	\item $\int \frac{dx}{a^2\cos^x-b^2\sin^2x}=\frac{1}{2ab}\ln|\frac{b\tan x+a}{b\tan x-a}|+C$
	\item $\int x\sin axdx=\frac{1}{a^2}\sin ax-\frac{x}{a}\cos ax+C$
	\item $\int x^2\sin axdx=-\frac{1}{a}x^2\cos ax+\frac{2}{a^2}x\sin ax+\frac{2}{a^3}\cos ax+C$
	\item $\int x\cos axdx=\frac{1}{a^2}\cos ax+\frac{1}{a}+C$
	\item $\int x^2\cos axdx=\frac{1}{a}x^2\sin ax+\frac{2}{a^2}x\cos ax-\frac{2}{a^3}\sin ax+C$
\end{itemize}
\subsection{含有反三角函数的积分（其中a>0）}
\begin{itemize}
	\item $\int \arcsin\frac{x}{a}=x\arcsin\frac{x}{a}+\sqrt{a^2-x^2}+C$
	\item $\int xarcsin\frac{x}{a}dx=\left(\frac{x^2}{2}-\frac{a^2}{3}\right)\arcsin\frac{x}{a}+\frac{x}{4}\sqrt{a^2-x^2}+C$
	\item $\int x^2\arcsin\frac{x}{a}dx=\frac{x^3}{3}\arcsin\frac{x}{a}-\frac{1}{9}\left(x^2+2a^2\right)\sqrt{a^2-x^2}+C$
	\item $$
	\item $$
	\item $$
	\item $$
	\item $$
	\item $$
\end{itemize}